Trie.fst
@@ -7,16 +7,17 @@ open TrieDataType
 open FStar.Classical.Sugar
 open Container
 
-type trie_array = raw (trie0 alphabet_size) alphabet_size
+type trie_array (n: u32pos) = raw (trie0 n) n
 
-let empty : trie0 alphabet_size = L
+let empty (n: u32pos) : trie0 n = L
 
 // ==========================
 //  Trie Operations
 // ==========================
 
-let rec mem (l : list b_nat) (t : trie0 alphabet_size) : Tot bool (decreases l) =
-  match t with
+let rec mem (#alph_size: u32pos) (l: list (b_nat alph_size)) (t: trie0 alph_size)
+  : Tot bool (decreases l)
+  = match t with
   | L -> false
   | N (a, is_t) ->
     match l with
@@ -26,31 +27,33 @@ let rec mem (l : list b_nat) (t : trie0 alphabet_size) : Tot bool (decreases l) 
       | L -> false
       | t' -> mem xs t'
 
-let empty_array : trie_array =
-  init alphabet_size (fun _ -> L)
+let empty_array (alph_size: u32pos) : trie_array alph_size =
+  init alph_size (fun _ -> L)
 
-let rec insert0 (l: list b_nat) (t : trie0 alphabet_size) : Tot (trie0 alphabet_size) (decreases l) =
-  match (t,l) with
-  | (L, []) -> N (empty_array, true)
+let rec insert0 (#alph_size: u32pos) (l: list (b_nat alph_size)) (t: trie0 alph_size)
+  : Tot (trie0 alph_size) (decreases l)
+  = match (t,l) with
+  | (L, []) -> N (empty_array alph_size, true)
   | (N (a, _), []) -> N (a, true)
-  | (L, x::xs) -> N (init alphabet_size (fun i -> if i = x then insert0 xs L else L), false)
+  | (L, x::xs) -> N (init alph_size (fun i -> if i = x then insert0 xs L else L), false)
   | (N (a, b), x::xs) ->
     let t' = index a (U32.uint_to_t x) in
     N (update a (U32.uint_to_t x) (insert0 xs t'), b)
 
-let rec is_empty' (a:trie_array) (i:b_nat)
+let rec is_empty' (#alph_size: u32pos) (a: trie_array alph_size) (i: b_nat alph_size)
   : Tot bool (decreases i)
-= if N? (index a (U32.uint_to_t i))
+  = if N? (index a (U32.uint_to_t i))
   then false
   else if i = 0
        then true
        else is_empty' a (i-1)
 
-let is_empty (a:trie_array) : bool
-  = is_empty' a ((U32.v alphabet_size) - 1)
+let is_empty (#alph_size: u32pos) (a:trie_array alph_size) : bool
+  = is_empty' #alph_size a ((U32.v alph_size) - 1)
 
-let rec delete0 (l: list b_nat) (t : trie0 alphabet_size) : Tot (trie0 alphabet_size) (decreases l) =
-  match (t,l) with
+let rec delete0 (#alph_size: u32pos) (l: list (b_nat alph_size)) (t: trie0 alph_size)
+  : Tot (trie0 alph_size) (decreases l)
+  = match (t,l) with
   | (L, _) -> L
   | (N (a, _), []) -> if is_empty a then L else N (a,false)
   | (N (a, is_t), x::xs) ->
@@ -70,16 +73,16 @@ let rec delete0 (l: list b_nat) (t : trie0 alphabet_size) : Tot (trie0 alphabet_
 
 // ---- insert Lemma ----
 
-let rec insert0_trie (l:list b_nat) (t:trie0 alphabet_size)
+let rec insert0_trie (#alph_size: u32pos) (l:list (b_nat alph_size)) (t: trie0 alph_size)
   : Lemma (requires is_trie t) (ensures is_trie (insert0 l t))
-  =
-  match (t,l) with
+  = match (t,l) with
   | (L,[]) -> ()
   | (_,[]) -> ()
   | (L,x::xs) -> insert0_trie xs L
   | (N (a, b), x::xs) -> insert0_trie xs (index a (U32.uint_to_t x))
 
-let insert (x:list b_nat) (t:trie) : trie
+let insert (#alph_size: u32pos) (x:list (b_nat alph_size)) (t:trie alph_size)
+  : trie alph_size
   =
   insert0_trie x t;
   insert0 x t
@@ -88,67 +91,67 @@ let insert (x:list b_nat) (t:trie) : trie
 
 // -- exists child node ==> not (is_empty a) --
 
-let rec del_lem_back2 (a:trie_array)
-                      (i':b_nat)
-                      (pf:squash (not (is_empty' a i')))
-  : Tot (squash (not (is_empty a))) (decreases (U32.v alphabet_size - i'))
+let rec del_lem_back2 (alph_size: u32pos) (a: trie_array alph_size)
+                      (i': b_nat alph_size)
+                      (pf: squash (not (is_empty' #alph_size a i')))
+  : Tot (squash (not (is_empty a))) (decreases (U32.v alph_size - i'))
   =
-  if i' = U32.v alphabet_size - 1
+  if i' = U32.v alph_size - 1
   then pf
   else let pf' : squash (not (is_empty' a (i'+1))) = () in
-       del_lem_back2 a (i'+1) pf'
+       del_lem_back2 alph_size a (i'+1) pf'
 
-let del_lem_back1 (a:trie_array)
-  : Lemma (requires (exists (i:b_nat).
+let del_lem_back1 (alph_size: u32pos) (a: trie_array alph_size)
+  : Lemma (requires (exists (i: b_nat alph_size).
                      N? (index a (U32.uint_to_t i))))
           (ensures not (is_empty a))
   =
-  let pf : squash (exists (i': b_nat). not (is_empty' a i')) = () in
+  let pf : squash (exists (i': b_nat alph_size). not (is_empty' a i')) = () in
   exists_elim
   #_
   #(fun i' -> not (is_empty' a i'))
   #(not (is_empty a))
   pf
-  (del_lem_back2 a)
+  (del_lem_back2 alph_size a)
 
-let del_lem_back (a:trie_array)
-  : Lemma ((exists (i:b_nat).
+let del_lem_back (alph_size: u32pos) (a: trie_array alph_size)
+  : Lemma ((exists (i: b_nat alph_size).
                     N? (index a (U32.uint_to_t i)))
            ==>
           (not (is_empty a)))
   =
-  implies_intro (exists (i:b_nat).
+  implies_intro (exists (i: b_nat alph_size).
                          N? (index a (U32.uint_to_t i)))
                 (fun pfp -> (not (is_empty a)))
-                (fun pfp -> del_lem_back1 a)
+                (fun pfp -> del_lem_back1 alph_size a)
 
 // -- exists child node <== not (is_empty a) --
 
-let rec del_lem' (a:trie_array) (i:b_nat)
+let rec del_lem' (alph_size: u32pos) (a: trie_array alph_size) (i: b_nat alph_size)
   : Lemma (requires not (is_empty' a i))
-          (ensures (exists (i:b_nat).
+          (ensures (exists (i: b_nat alph_size).
                             N? (index a (U32.uint_to_t i))))
   =
   if N? (index a (U32.uint_to_t i))
   then ()
   else if i = 0
       then ()
-      else del_lem' a (i-1)
+      else del_lem' alph_size a (i-1)
 
-let del_lem (a:trie_array)
+let del_lem (alph_size: u32pos) (a: trie_array alph_size)
   : Lemma (requires not (is_empty a))
-          (ensures (exists (i:b_nat).
+          (ensures (exists (i: b_nat alph_size).
                             N? (index a (U32.uint_to_t i))))
-  = del_lem' a (U32.v alphabet_size - 1)
+  = del_lem' alph_size a (U32.v alph_size - 1)
 
 // ---- delete Lemma ----
 
-let rec delete0_trie (l:list b_nat) (t:trie0 alphabet_size)
+let rec delete0_trie (#alph_size: u32pos) (l: list (b_nat alph_size)) (t: trie0 alph_size)
   : Lemma (requires is_trie t) (ensures is_trie (delete0 l t))
   =
   match (t,l) with
   | (L,_) -> ()
-  | (N (a,_), []) -> if is_empty a then () else del_lem a
+  | (N (a,_), []) -> if is_empty a then () else del_lem alph_size a
   | (N (a,is_t), x::xs) ->
       match index a (U32.uint_to_t x) with
       | L -> ()
@@ -157,10 +160,11 @@ let rec delete0_trie (l:list b_nat) (t:trie0 alphabet_size)
         | L -> let N (a',b') = N (update a (U32.uint_to_t x) L , is_t)
                in if is_empty a' && not is_t
                   then ()
-                  else if is_t then () else del_lem a'
+                  else if is_t then () else del_lem alph_size a'
         | t'' -> delete0_trie xs t'
 
-let delete (x:list b_nat) (t:trie) : trie
+let delete (#alph_size: u32pos) (x: list (b_nat alph_size)) (t: trie alph_size)
+  : trie alph_size
   =
   delete0_trie x t;
   delete0 x t
@@ -170,43 +174,44 @@ let delete (x:list b_nat) (t:trie) : trie
 // ==========================
 
 let models
-  (xs : trie0 alphabet_size)
-  (ss : TSet.set (list b_nat))
+  (#alph_size: u32pos)
+  (xs: trie0 alph_size)
+  (ss: TSet.set (list (b_nat alph_size)))
   : GTot prop
   =
-  forall (x: list b_nat).
+  forall (x: list (b_nat alph_size)).
          mem x xs <==> TSet.mem x ss
 
-let empty_ok_lem (_:unit) : Lemma (models empty TSet.empty)
+let empty_ok_lem (#alph_size: u32pos) (_:unit) : Lemma (models (empty alph_size) TSet.empty)
   = ()
 
-let rec is_empty_lem (t:trie{N? t})
-  : squash (exists (l:list b_nat) . mem l t) 
+let rec is_empty_lem (#alph_size: u32pos) (t: trie alph_size{N? t})
+  : squash (exists (l: list (b_nat alph_size)) . mem l t)
   =
   match t with
   | N (a,true) -> assert(mem [] t)
   | N (a,false) ->
-    let pf : squash (exists (i:b_nat).
+    let pf: squash (exists (i: b_nat alph_size).
                              N? (index a (U32.uint_to_t i))) = ()
     in exists_elim
-       #b_nat
+       #(b_nat alph_size)
        #(fun i -> N? (index a (U32.uint_to_t i)))
-       #(exists (l:list b_nat) . mem l t)
+       #(exists (l: list (b_nat alph_size)) . mem l t)
        pf
        (fun i pfx -> (
                       is_empty_lem (index a (U32.uint_to_t i));
-                      assert(exists (l:list b_nat). mem (i::l) t)
+                      assert(exists (l: list (b_nat alph_size)). mem (i::l) t)
                       )
        )
 
-let is_empty_ok (xs:trie)
+let is_empty_ok (#alph_size: u32pos) (xs: trie alph_size)
   : Lemma (models xs TSet.empty <==> L? xs)
   =
   match xs with
   | L -> ()
   | N (_,_) -> is_empty_lem xs
 
-let rec mem_insert (t:trie) (l: list b_nat)
+let rec mem_insert (#alph_size: u32pos) (t: trie alph_size) (l: list (b_nat alph_size))
   : Lemma (mem l (insert l t))
   =
   match (t,l) with
@@ -214,7 +219,11 @@ let rec mem_insert (t:trie) (l: list b_nat)
   | (L, x::xs) -> mem_insert t xs
   | (N (a,is_t), x::xs) -> mem_insert (index a (U32.uint_to_t x)) xs
 
-let rec ins_ok_lem1 (t:trie) (l: list b_nat) (l':(list b_nat){mem l' t})
+let rec ins_ok_lem1
+  (#alph_size: u32pos)
+  (t: trie alph_size)
+  (l: list (b_nat alph_size))
+  (l': (list (b_nat alph_size)){mem l' t})
   : Tot (squash (mem l' (insert l t))) (decreases l')
   =
   match (t,l,l') with
@@ -230,7 +239,11 @@ let rec ins_ok_lem1 (t:trie) (l: list b_nat) (l':(list b_nat){mem l' t})
          )
     else ()
 
-let rec ins_ok_lem2 (t:trie) (l: list b_nat) (l':(list b_nat){not (mem l' t) /\ (l <> l')})
+let rec ins_ok_lem2
+  (#alph_size: u32pos)
+  (t: trie alph_size)
+  (l: list (b_nat alph_size))
+  (l': (list (b_nat alph_size)){not (mem l' t) /\ (l <> l')})
   : Tot (squash (not (mem l' (insert l t)))) (decreases l')
   =
   match (t,l,l') with
@@ -243,7 +256,11 @@ let rec ins_ok_lem2 (t:trie) (l: list b_nat) (l':(list b_nat){not (mem l' t) /\ 
     then ins_ok_lem2 (index a (U32.uint_to_t x)) xs ys
     else ()
 
-let ins_ok_lem (x:list b_nat) (xs:trie) (ss : TSet.set (list b_nat))
+let ins_ok_lem
+  (#alph_size: u32pos)
+  (x: list (b_nat alph_size))
+  (xs: trie alph_size)
+  (ss: TSet.set (list (b_nat alph_size)))
   : Lemma (requires xs `models` ss)
           (ensures  insert x xs
                      `models`
@@ -251,15 +268,15 @@ let ins_ok_lem (x:list b_nat) (xs:trie) (ss : TSet.set (list b_nat))
   =
   mem_insert xs x;
 
-  forall_intro (l:(list b_nat){mem l xs})
+  forall_intro (l: (list (b_nat alph_size)){mem l xs})
                (fun l' -> mem l' (insert x xs))
                (ins_ok_lem1 xs x);
 
-  forall_intro (l:(list b_nat){not (mem l xs) /\ (l <> x)})
+  forall_intro (l: (list (b_nat alph_size)){not (mem l xs) /\ (l <> x)})
                (fun l' -> not (mem l' (insert x xs)))
                (ins_ok_lem2 xs x)
 
-let rec mem_delete (t:trie) (l:list b_nat)
+let rec mem_delete (#alph_size: u32pos) (t: trie alph_size) (l: list (b_nat alph_size))
   : Lemma (not (mem l (delete l t)))
   =
   match (t,l) with
@@ -273,7 +290,11 @@ let rec mem_delete (t:trie) (l:list b_nat)
         | L -> ()
         | t'' -> mem_delete t' xs
 
-let rec del_ok_lem1 (t:trie) (l:list b_nat) (l':(list b_nat){not (mem l' t)})
+let rec del_ok_lem1
+  (#alph_size: u32pos)
+  (t: trie alph_size)
+  (l: list (b_nat alph_size))
+  (l': (list (b_nat alph_size)){not (mem l' t)})
   : Tot (squash (not (mem l' (delete l t))))
   =
   match (t,l,l') with
@@ -292,14 +313,18 @@ let rec del_ok_lem1 (t:trie) (l:list b_nat) (l':(list b_nat){not (mem l' t)})
          )
     else ()
 
-let del_ok_lem2' (t:trie{N? t}) (l:(list b_nat){Cons? l})
+let del_ok_lem2' (#alph_size: u32pos) (t: trie alph_size{N? t}) (l: (list (b_nat alph_size)){Cons? l})
   : Lemma (requires (let N (a,_) = t in is_empty a))
           (ensures not (mem l t))
   =
   match (t,l) with
-  | (N (a,_),_) -> del_lem_back a
+  | (N (a,_),_) -> del_lem_back alph_size a
 
-let rec del_ok_lem2 (t:trie) (l:list b_nat) (l':(list b_nat){(mem l' t) /\ (l <> l')})
+let rec del_ok_lem2
+  (#alph_size: u32pos)
+  (t: trie alph_size)
+  (l: list (b_nat alph_size))
+  (l': (list (b_nat alph_size)){(mem l' t) /\ (l <> l')})
   : Tot (squash (mem l' (delete l t)))
   =
   match (t,l,l') with
@@ -321,10 +346,14 @@ let rec del_ok_lem2 (t:trie) (l:list b_nat) (l':(list b_nat){(mem l' t) /\ (l <>
     else (
           match index a (U32.uint_to_t x) with
           | L -> ()
-          | t' -> del_lem_back (update a (U32.uint_to_t x) L)
+          | t' -> del_lem_back alph_size (update a (U32.uint_to_t x) L)
          )
 
-let del_ok_lem (x:list b_nat) (t:trie) (ss: TSet.set (list b_nat))
+let del_ok_lem
+  (#alph_size: u32pos)
+  (x: list (b_nat alph_size))
+  (t: trie alph_size)
+  (ss: TSet.set (list (b_nat alph_size)))
   : Lemma (requires t `models` ss)
           (ensures delete x t
                    `models`
@@ -332,18 +361,18 @@ let del_ok_lem (x:list b_nat) (t:trie) (ss: TSet.set (list b_nat))
   =
   mem_delete t x;
 
-  //assume(forall (l:(list b_nat){not (mem t l)}). not (mem (delete x t) l));
-  forall_intro (l:(list b_nat){not (mem l t)})
+  //assume(forall (l: (list (b_nat alph_size)){not (mem t l)}). not (mem (delete x t) l));
+  forall_intro (l: (list (b_nat alph_size)){not (mem l t)})
                (fun l' -> not (mem l' (delete x t)))
                (del_ok_lem1 t x);
   
-  //assume(forall (l:(list b_nat){(mem t l) /\ (l <> x)}). (mem (delete x t) l));
-  forall_intro (l:(list b_nat){(mem l t) /\ (l <> x)})
+  //assume(forall (l: (list (b_nat alph_size)){(mem t l) /\ (l <> x)}). (mem (delete x t) l));
+  forall_intro (l: (list (b_nat alph_size)){(mem l t) /\ (l <> x)})
                (fun l' -> mem l' (delete x t))
                (del_ok_lem2 t x)
 
-instance tries_are_containers0
-  : container0 (list b_nat) trie = {
+instance tries_are_containers0 (#alph_size: u32pos)
+  : container0 (list (b_nat alph_size)) (trie alph_size) = {
     empty = L;
     is_empty = L?;
 
@@ -352,18 +381,18 @@ instance tries_are_containers0
     del = delete;
   }
 
-instance tries_are_container_laws
-  : container_laws (list b_nat) trie tries_are_containers0 = {
+instance tries_are_container_laws (#alph_size: u32pos)
+  : container_laws (list (b_nat alph_size)) (trie alph_size) tries_are_containers0 = {
     models = models;
-    empty_ok = empty_ok_lem;
+    empty_ok = empty_ok_lem #alph_size;
     is_empty_ok = is_empty_ok;
     mem_ok = (fun _ _ _ -> ());
     ins_ok = ins_ok_lem;
     del_ok = del_ok_lem;
 }
 
-instance tries_are_containers
-  : container (list b_nat) trie = {
+instance tries_are_containers (#alph_size: u32pos)
+  : container (list (b_nat alph_size)) (trie alph_size) = {
     ops = tries_are_containers0;
     laws = tries_are_container_laws;
   }
