TrieDataType.fst
@@ -4,37 +4,33 @@ open FStar.Vector
 module U32 = FStar.UInt32
 module U = FStar.UInt
 
-let alphabet_size : U32.t = U32.uint_to_t 26
-
 // b_nat represents a bounded natural that can fit in 32 bits
-type b_nat = x:nat{x < U32.v alphabet_size /\ U.size x 32}
+type b_nat (alph_size: U32.t) = x: nat{x < U32.v alph_size /\ U.size x 32}
 
-let functio (b_nat) : bool = true
-
-let v : b_nat = 25
+type u32pos = (n: U32.t{U32.v n > 0})
 
 noeq
-type trie0 (n : U32.t) =
+type trie0 (n: U32.t) =
   | L
   | N of raw (trie0 n) n & bool
 
-let index_dec (#a:Type) (l:len_t) (v:raw a l) (i : U32.t{U32.v i < U32.v l})
+let index_dec (#a: Type) (l: len_t) (v: raw a l) (i: U32.t{U32.v i < U32.v l})
   : Lemma (index v i << v)
           [SMTPat (index v i)]
   = admit()
 
-let rec is_trie (t:trie0 alphabet_size) : Tot prop
+let rec is_trie (#alph_size: u32pos) (t: trie0 alph_size) : Tot prop
   =
   match t with
   | L -> true
   | N (a,true) ->
-    (forall (i:b_nat).
+    (forall (i:b_nat alph_size).
       is_trie (index a (U32.uint_to_t i)))
   | N (a,false) ->
-    (forall (i:b_nat).
+    (forall (i:b_nat alph_size).
       is_trie (index a (U32.uint_to_t i)))
     /\
-    (exists (i:b_nat).
+    (exists (i:b_nat alph_size).
         N? (index a (U32.uint_to_t i)))
 
-type trie = t:(trie0 alphabet_size){is_trie t}
+type trie (alph_size: u32pos) = t: (trie0 alph_size){is_trie t}
