Trie.fsti
@@ -3,11 +3,11 @@ module Trie
 open Container
 open TrieDataType
 
-instance val tries_are_containers0
-  : container0 (list b_nat) trie
+instance val tries_are_containers0 (#alph_size: u32pos)
+  : container0 (list (b_nat alph_size)) (trie alph_size)
 
-instance val tries_are_container_laws
-  : container_laws (list b_nat) trie tries_are_containers0
+instance val tries_are_container_laws (#alph_size: u32pos)
+  : container_laws (list (b_nat alph_size)) (trie alph_size) tries_are_containers0
 
-instance val tries_are_containers
-  : container (list b_nat) trie
+instance val tries_are_containers (#alph_size: u32pos)
+  : container (list (b_nat alph_size)) (trie alph_size)
